

Symbolic Artificial Intelligence (COMP3008)

Lecture 6: Propositional Reasoning

3 November 2025

Daniel Karapetyan

`daniel.karapetyan@nottingham.ac.uk`

Updates

Coursework Project

- Released on 28th October
- There was a minor mistake in the code of the automated test; if you made a copy of the notebook before Friday evening, please update the code of the test
- Deadline 20th November 15:00
- Standard late penalty applies (5 points per day, up to two days)
- Will release the submission system closer to the deadline (to avoid overloading Moodle)
- Expected to spend in the order of 70 hours in total (during the computing classes and in your own time)
- Compulsory interview

Early Module Feedback

- Generally positive
- Pace of delivery seems to be OK
- Many of you found the worksheets helpful and fun
- Many of you found the quizzes helpful
- Requests for more in-class interactive sessions (Slido and review of exercises)
- A few concerns about the worksheets:
 - Do not align with the lecture materials
 - Difficult
 - There were several requests of worksheet solutions
- Immediate changes based on your feedback:
 - Will do more in-class activities
 - I have released the model answers to the worksheets today (see Moodle)

Propositional Logic and CNF

Propositional Logic (Recap)

- Propositional logic is a subset of FOL
- It is 'FOL without the domain of discourse'
- Example of a propositional logic sentence: $P \rightarrow (Q \wedge \neg R)$
- Any propositional formula can be expressed in the standard forms: CNF or DNF
- The above sentence in CNF: $(\neg P \vee Q) \wedge (\neg P \vee \neg R)$

Conversion into CNF

1 Get rid of \leftrightarrow and \rightarrow :

- Replace every $(\alpha \leftrightarrow \beta)$ with $((\alpha \rightarrow \beta) \wedge (\beta \rightarrow \alpha))$
- Replace every $(\alpha \rightarrow \beta)$ with $(\neg\alpha \vee \beta)$

Now, the formula includes only \wedge , \vee and \neg operators

2 Push \neg inside brackets:

- Replace every $\neg(\alpha \wedge \beta \wedge \dots)$ with $(\neg\alpha \vee \neg\beta \vee \dots)$
- Replace every $\neg(\alpha \vee \beta \vee \dots)$ with $(\neg\alpha \wedge \neg\beta \wedge \dots)$
- Replace every $\neg\neg\alpha$ with α

Now \neg appears only next to literals

3 Example of the formula at this stage:

$$(A \wedge (B \vee (C \wedge \neg A))) \vee (\neg B \wedge C)$$

- Replace every $((\alpha \wedge \beta) \vee \gamma)$ with $((\alpha \vee \gamma) \wedge (\beta \vee \gamma))$
- Open unnecessary brackets, e.g. $(\alpha \vee \beta) \vee \gamma$ becomes $\alpha \vee \beta \vee \gamma$

4 Replace every $(\alpha \wedge \alpha)$ and $(\alpha \vee \alpha)$ with α

CNF and DNF size

- Distribution of \vee increases the size of the formula

- E.g. $(X_1 \wedge X_2 \wedge X_3) \vee (Y_1 \wedge Y_2 \wedge Y_3)$

looks as follows in CNF:

$$(X_1 \vee Y_1) \wedge (X_1 \vee Y_2) \wedge (X_1 \vee Y_3) \wedge (X_2 \vee Y_1) \wedge (X_2 \vee Y_2) \\ \wedge (X_2 \vee Y_3) \wedge (X_3 \vee Y_1) \wedge (X_3 \vee Y_2) \wedge (X_3 \vee Y_3)$$

Here, the transformation increased the formula size **quadratically**

- **How much can it increase the formula size in the worst case?**

CNF and DNF size

- Distribution of \vee increases the size of the formula

- E.g. $(X_1 \wedge X_2 \wedge X_3) \vee (Y_1 \wedge Y_2 \wedge Y_3)$

looks as follows in CNF:

$$(X_1 \vee Y_1) \wedge (X_1 \vee Y_2) \wedge (X_1 \vee Y_3) \wedge (X_2 \vee Y_1) \wedge (X_2 \vee Y_2) \\ \wedge (X_2 \vee Y_3) \wedge (X_3 \vee Y_1) \wedge (X_3 \vee Y_2) \wedge (X_3 \vee Y_3)$$

Here, the transformation increased the formula size **quadratically**

- **How much can it increase the formula size in the worst case?**

Some other formulas such as

$$(X_1 \wedge Y_1) \vee (X_2 \wedge Y_2) \vee (X_3 \wedge Y_3) \vee \dots$$

may increase **exponentially** when converted into CNF (see https://en.wikipedia.org/wiki/Conjunctive_normal_form#Conversion_into_CNF for details)

- This is a problem for reasoning systems that require the formula being in CNF
- DNF has a similar conversion procedure, which may also yield a formula of exponential size

Resolution for Propositional Case

Clausal representation

- Since CNF has a simple structure, it can be written in a compact form called *clausal representation*

- Recall that a formula in CNF is a set of clauses:

$$\underbrace{(A \vee \neg B)}_{\text{Clause 1}} \wedge \underbrace{(\neg C \vee D)}_{\text{Clause 2}} \wedge \underbrace{(\neg A \vee B \vee C)}_{\text{Clause 3}}$$

- Each clause is a set of literals, e.g.:

$$(\underbrace{A}_{\text{Literal 1}} \vee \underbrace{\neg B}_{\text{Literal 2}})$$

- Each literal is either a predicate or its negation

- We use:

- Curly brackets for formulas
- Square brackets for clauses
- \neg for negation

- E.g., the above formula can be written as

$$\{[A, \bar{B}], [\bar{C}, D], [\bar{A}, B, C]\}$$

Clausal representation

- Clausal representation is used for convenience only; it is exactly equivalent to the usual form
- Clausal representation allows us to conveniently handle formulas as mathematical objects (sets of sets)
- $[]$ stands for

Clausal representation

- Clausal representation is used for convenience only; it is exactly equivalent to the usual form
- Clausal representation allows us to conveniently handle formulas as mathematical objects (sets of sets)
- $[]$ stands for FALSE as the neutral element for disjunction is FALSE: $X \vee \text{FALSE} \leftrightarrow X$
- $\{\}$ stands for

Clausal representation

- Clausal representation is used for convenience only; it is exactly equivalent to the usual form
- Clausal representation allows us to conveniently handle formulas as mathematical objects (sets of sets)
- $[]$ stands for FALSE as the neutral element for disjunction is FALSE: $X \vee \text{FALSE} \leftrightarrow X$
- $\{\}$ stands for TRUE as the neutral element for conjunction is TRUE: $X \wedge \text{TRUE} \leftrightarrow X$
- $\{[]\}$ stands for

Clausal representation

- Clausal representation is used for convenience only; it is exactly equivalent to the usual form
- Clausal representation allows us to conveniently handle formulas as mathematical objects (sets of sets)
- $[]$ stands for FALSE as the neutral element for disjunction is FALSE: $X \vee \text{FALSE} \leftrightarrow X$
- $\{\}$ stands for TRUE as the neutral element for conjunction is TRUE: $X \wedge \text{TRUE} \leftrightarrow X$
- $\{[]\}$ stands for FALSE because it is $\{\text{FALSE}\}$

Resolution rule of inference

Let P be a literal and α and β be sets of literals

Having two clauses:

$[P, \alpha]$ and $[\bar{P}, \beta]$

we can *infer* a new clause $[\alpha, \beta]$, called *resolvent*

This process is called *resolution*

Indeed, if P is FALSE then α has to be TRUE; if P is TRUE then β has to be TRUE; hence, either α or β is TRUE

Example

Let us consider two clauses:

$[A, B, \bar{C}]$ and $[\bar{A}, D]$
 $\underbrace{\hspace{1.5cm}}_{\alpha} \quad \underbrace{\hspace{1.5cm}}_{\beta}$

Then the resolvent is $[B, \bar{C}, D]$, and it is entailed by the two given clauses

Derivation

Note that adding the resolvent $[\alpha, \beta]$ to the formula does not change its evaluation

- Indeed, the resolvent is entailed by the input clauses

Derivation of a clause c from a set of clauses S is a process of inferring clauses c_1, c_2, \dots, c_n , where $c = c_n$ and c_i is inferred from $S \cup \{c_1, c_2, \dots, c_{i-1}\}$

We write $S \vdash c$ if c can be derived from S

Special case resolvent

For clauses $[P]$ and $[\bar{P}]$, the resolvent is $[]$ because $\alpha = \beta = \emptyset$

Recall that $[]$ evaluates as FALSE; then clauses $[P]$ and $[\bar{P}]$ entail FALSE

Indeed:

$$P \wedge \neg P \models \text{FALSE}$$

Derivation and entailment

Recall that the resolvent is entailed by the original clauses

Hence if $S \vdash c$ then $S \models c$

The opposite is not necessarily true, e.g.

$$P \models P \vee Q$$

but you will never infer $P \vee Q$ from P

In other words, knowing whether $S \vdash \gamma$ is **not always enough** to know whether $S \models \gamma$

Refutation

However, there is a trick!

It is possible to demonstrate that if S is unsatisfiable then $S \vdash []$

We say that the inference mechanism is *refutation-complete* – it guarantees to prove or disprove that S is unsatisfiable

Negation of the hypothesis

A reasoning system needs to verify if $S \models \gamma$

If we have a refutation-complete inference mechanism, we can use the following observation:

$S \models \gamma$ if and only if $S \wedge \neg\gamma$ is unsatisfiable

Indeed,

- If $S \wedge \neg\gamma$ is unsatisfiable then every interpretation that satisfies S also satisfies γ
- If $S \wedge \neg\gamma$ is satisfiable then there is an interpretation that satisfies S but does not satisfy γ

Then our goal is to verify if $S \cup \{\neg\gamma\}$ is unsatisfiable, which can be done using a refutation-complete inference mechanism

Reasoning system based on resolution

Algorithm 1: Reasoning procedure for propositional logic

input : S (knowledge base in CNF), γ (the hypothesis)

```
1 Let  $S'$  be  $\neg\gamma$  in CNF;  
2 Let  $S \leftarrow S \cup S'$  (i.e. add the negation of the hypothesis to the KB);  
3 Loop  
4   if  $[] \in S$  then  
5     return ENTAILED;  
6   if exist  $[P, \alpha], [\bar{P}, \beta] \in S$  such that  $[\alpha, \beta] \notin S$  then  
7     Add clause  $[\alpha, \beta]$  to  $S$ ;  
8   else  
9     return NOT ENTAILED;
```

Summary: reasoning in propositional logic

- FOL is semi-decidable
- To achieve decidability, we can restrict the language: propositional logic
- CNF – to unify the representation
- CNF of a small formula may be exponentially big!
- Resolution rule of inference (one of many possible) but we know it is sufficient
- Every time we apply the resolution rule of inference, we create a new clause that is entailed by our original sentence:
 - Given a sentence (set of sentences, knowledge base) – S
 - By applying the resolution rule of inference, obtain a new clause c
 - Guaranteed that $S \models c$
 - Then $S \wedge c \leftrightarrow S$
 - We can replace S with $S \wedge c$

Refutation-complete reasoning system

- The resolution-based reasoning system may never arrive to our hypothesis
- But it is **refutation-complete**

Guaranteed to arrive to an empty clause if the sentence is unsatisfiable

- How can we exploit this to prove or disprove that $KB \models \gamma$?
 - Negate γ
 - Add $\neg\gamma$ to KB
 - Use resolution-based system to check if $KB \wedge \neg\gamma$ infer $[]$
 - If $KB \wedge \neg\gamma \vdash []$ then $KB \wedge \neg\gamma$ is unsatisfiable, hence every interpretation \mathcal{I} that satisfies S also satisfies γ ; we conclude that $KB \models \gamma$
 - If $KB \wedge \neg\gamma \not\vdash []$ then $KB \wedge \neg\gamma$ is satisfiable, hence there is an interpretation \mathcal{I} that satisfies S but does not satisfy γ ; we conclude that $KB \not\models \gamma$
 - (This is why we keep revising the definitions of entailment, satisfiability, etc.)

DPLL Algorithm

SAT – recap

- SAT is the problem of finding an interpretation that satisfies a given sentence in CNF (or proving that the sentence is unsatisfiable)
- Can be solved by inference: if $S \vdash \perp$ then S is unsatisfiable
- If S is satisfiable, can also find a specific interpretation; for example
 - if $S \wedge [A] \vdash \perp$ then let $A = \text{FALSE}$
 - if $S \wedge [A] \not\vdash \perp$ then let $A = \text{TRUE}$
- However, a purpose-build solver for SAT may (and does in practice) perform better

DPLL algorithm – background

Most of the modern SAT solvers are based on the DPLL algorithm, named after its creators Davis, Putnam, Logemann and Loveland

- Let S be our (finite) knowledge base in CNF
- Observe that S involves a finite number of propositional variables
- We can potentially try every combination of their values
 - If we find a combination that satisfies S then we solved the problem
 - If we did not find any combination that satisfies S then S is unsatisfiable
- In practice, we might not need to enumerate all possible combinations
 - Once we have a partial assignment of values, we may already be able to conclude that this partial assignment does not satisfy S
 - For example, in $\{[A, \overline{B}], [\overline{A}, C], [D]\}$ setting $D = \text{FALSE}$ makes the formula unsatisfiable; then there is no need to try all combinations of A , B and C with $D = \text{FALSE}$

DPLL algorithm – concept

- DPLL uses *Depth-First Search* (DFS)
- It selects a single propositional variable and then splits the search into two branches: when this variable is TRUE and when it is FALSE
- Knowing the value of a propositional variable, we can simplify the formula
- If the simplified formula contains an empty clause, it is unsatisfiable and no further search in this branch is needed

DPLL Algorithm

Algorithm 2: DPLL Algorithm (Simplified)

input : Set of clauses S

output: TRUE if S is satisfiable and FALSE otherwise

```
1 if  $[] \in S$  then
2   | return FALSE;
3 else if  $S$  is empty then
4   | return TRUE;
5 else
6   | Select a propositional variable  $A$  used in  $S$ ;
7   |  $S' \leftarrow \text{Propagate}(S, A)$ ;
8   |  $S'' \leftarrow \text{Propagate}(S, \overline{A})$ ;
9   | return  $DPLL(S') \vee DPLL(S'')$ ;
```

The real algorithm also keeps record of the assignments of values to the propositional variables

DPLL Algorithm – Propagation

Algorithm 3: Propagate(S, A)

input : Set of clauses S ; literal A (variable or negated variable)

output: Set of clauses S'

```
1 Let  $S' \leftarrow \emptyset$ ;  
2 for  $c \in S$  do  
3   if  $A \in c$  then  
4     | Skip this clause (we don't need it as it evaluates to TRUE);  
5   else if  $\bar{A} \in c$  then  
6     |  $S' \leftarrow S' \cup \{c \setminus \{\bar{A}\}\}$ ;  
7     | (Since  $\bar{A} = \text{FALSE}$ , we can remove it but keep the clause)  
8   else  
9     |  $S' \leftarrow S' \cup \{c\}$ ;  
10    | (This clause is unaffected by the assignment)  
11 return  $S'$ 
```

Speed Ups of DPLL

DPLL also implements several speed ups

- If a clause consists of one literal only, we can set this literal to true and then propagate
- If a propositional variable appears only in one polarity (i.e. either as A only, or as \bar{A} only), we can set its value (to TRUE or FALSE, respectively) and propagate
- Performance of the algorithm is extremely dependent on the choice of the propositional variable A in line 6 of Algorithm 2; intelligent heuristics are used to select propositional variable A

DPLL Algorithm – example

KB: $\{[A, B, C], [\bar{A}, B], [\bar{B}, C], [\bar{B}, \bar{C}]\}$

Reminder: this is equivalent to

$$(A \vee B \vee C) \wedge (\neg A \vee B) \wedge (\neg B \vee C) \wedge (\neg B \vee \neg C)$$

DPLL Algorithm – example

KB: $\{[A, B, C], [\bar{A}, B], [\bar{B}, C], [\bar{B}, \bar{C}]\}$

Reminder: this is equivalent to

$$(A \vee B \vee C) \wedge (\neg A \vee B) \wedge (\neg B \vee C) \wedge (\neg B \vee \neg C)$$

Assume that the branching heuristic selects A :

DPLL Algorithm – example

KB: $\{[A, B, C], [\bar{A}, B], [\bar{B}, C], [\bar{B}, \bar{C}]\}$

Reminder: this is equivalent to

$$(A \vee B \vee C) \wedge (\neg A \vee B) \wedge (\neg B \vee C) \wedge (\neg B \vee \neg C)$$

Assume that the branching heuristic selects A :

Let $A = \text{TRUE}$:

DPLL Algorithm – example

KB: $\{[A, B, C], [\bar{A}, B], [\bar{B}, C], [\bar{B}, \bar{C}]\}$

Reminder: this is equivalent to

$$(A \vee B \vee C) \wedge (\neg A \vee B) \wedge (\neg B \vee C) \wedge (\neg B \vee \neg C)$$

Assume that the branching heuristic selects A :

Let $A = \text{TRUE}$:

■ Propagation: $\{[B], [\bar{B}, C], [\bar{B}, \bar{C}]\}$

DPLL Algorithm – example

$$\text{KB: } \{[A, B, C], [\bar{A}, B], [\bar{B}, C], [\bar{B}, \bar{C}]\}$$

Reminder: this is equivalent to

$$(A \vee B \vee C) \wedge (\neg A \vee B) \wedge (\neg B \vee C) \wedge (\neg B \vee \neg C)$$

Assume that the branching heuristic selects A :

Let $A = \text{TRUE}$:

- Propagation: $\{[B], [\bar{B}, C], [\bar{B}, \bar{C}]\}$
- By speed-up, the first clause consists of only one literal; we set $B = \text{TRUE}$

DPLL Algorithm – example

$$\text{KB: } \{[A, B, C], [\bar{A}, B], [\bar{B}, C], [\bar{B}, \bar{C}]\}$$

Reminder: this is equivalent to

$$(A \vee B \vee C) \wedge (\neg A \vee B) \wedge (\neg B \vee C) \wedge (\neg B \vee \neg C)$$

Assume that the branching heuristic selects A :

Let $A = \text{TRUE}$:

- Propagation: $\{[B], [\bar{B}, C], [\bar{B}, \bar{C}]\}$
- By speed-up, the first clause consists of only one literal; we set $B = \text{TRUE}$
- Propagation: $\{[C], [\bar{C}]\}$

DPLL Algorithm – example

$$\text{KB: } \{[A, B, C], [\bar{A}, B], [\bar{B}, C], [\bar{B}, \bar{C}]\}$$

Reminder: this is equivalent to

$$(A \vee B \vee C) \wedge (\neg A \vee B) \wedge (\neg B \vee C) \wedge (\neg B \vee \neg C)$$

Assume that the branching heuristic selects A :

Let $A = \text{TRUE}$:

- Propagation: $\{[B], [\bar{B}, C], [\bar{B}, \bar{C}]\}$
- By speed-up, the first clause consists of only one literal; we set $B = \text{TRUE}$
- Propagation: $\{[C], [\bar{C}]\}$
- By speed-up, the first clause consists of only one literal; we set $C = \text{TRUE}$

DPLL Algorithm – example

KB: $\{[A, B, C], [\bar{A}, B], [\bar{B}, C], [\bar{B}, \bar{C}]\}$

Reminder: this is equivalent to

$$(A \vee B \vee C) \wedge (\neg A \vee B) \wedge (\neg B \vee C) \wedge (\neg B \vee \neg C)$$

Assume that the branching heuristic selects A :

Let $A = \text{TRUE}$:

- Propagation: $\{[B], [\bar{B}, C], [\bar{B}, \bar{C}]\}$
- By speed-up, the first clause consists of only one literal; we set $B = \text{TRUE}$
- Propagation: $\{[C], [\bar{C}]\}$
- By speed-up, the first clause consists of only one literal; we set $C = \text{TRUE}$
- Propagation: $\{[[]]\}$

DPLL Algorithm – example

KB: $\{[A, B, C], [\bar{A}, B], [\bar{B}, C], [\bar{B}, \bar{C}]\}$

Reminder: this is equivalent to

$$(A \vee B \vee C) \wedge (\neg A \vee B) \wedge (\neg B \vee C) \wedge (\neg B \vee \neg C)$$

Assume that the branching heuristic selects A :

Let $A = \text{TRUE}$:

- Propagation: $\{[B], [\bar{B}, C], [\bar{B}, \bar{C}]\}$
- By speed-up, the first clause consists of only one literal; we set $B = \text{TRUE}$
- Propagation: $\{[C], [\bar{C}]\}$
- By speed-up, the first clause consists of only one literal; we set $C = \text{TRUE}$
- Propagation: $\{[[]]\}$
- Conclusion: this branch is unsatisfiable

KB: $\{[A, B, C], [\bar{A}, B], [\bar{B}, C], [\bar{B}, \bar{C}]\}$

Let $A = \text{FALSE}$:

KB: $\{[A, B, C], [\bar{A}, B], [\bar{B}, C], [\bar{B}, \bar{C}]\}$

Let $A = \text{FALSE}$:

- Propagation: $\{[B, C], [\bar{B}, C], [\bar{B}, \bar{C}]\}$

Assume that the branching heuristic selects B :

- Let $B = \text{TRUE}$:

- Propagation: $\{[C], [\bar{C}]\}$

KB: $\{[A, B, C], [\bar{A}, B], [\bar{B}, C], [\bar{B}, \bar{C}]\}$

Let $A = \text{FALSE}$:

- Propagation: $\{[B, C], [\bar{B}, C], [\bar{B}, \bar{C}]\}$

Assume that the branching heuristic selects B :

- Let $B = \text{TRUE}$:

- Propagation: $\{[C], [\bar{C}]\}$

- By speed-up, the first clause consists of only one literal; we set $C = \text{TRUE}$

KB: $\{[A, B, C], [\bar{A}, B], [\bar{B}, C], [\bar{B}, \bar{C}]\}$

Let $A = \text{FALSE}$:

- Propagation: $\{[B, C], [\bar{B}, C], [\bar{B}, \bar{C}]\}$

Assume that the branching heuristic selects B :

- Let $B = \text{TRUE}$:

- Propagation: $\{[C], [\bar{C}]\}$

- By speed-up, the first clause consists of only one literal; we set $C = \text{TRUE}$

- Propagation: $\{[]\}$

KB: $\{[A, B, C], [\bar{A}, B], [\bar{B}, C], [\bar{B}, \bar{C}]\}$

Let $A = \text{FALSE}$:

- Propagation: $\{[B, C], [\bar{B}, C], [\bar{B}, \bar{C}]\}$

Assume that the branching heuristic selects B :

- Let $B = \text{TRUE}$:

- Propagation: $\{[C], [\bar{C}]\}$

- By speed-up, the first clause consists of only one literal; we set $C = \text{TRUE}$

- Propagation: $\{[]\}$

- Conclusion: this branch is unsatisfiable

- Let $B = \text{FALSE}$:

- Propagation: $\{[C]\}$

KB: $\{[A, B, C], [\bar{A}, B], [\bar{B}, C], [\bar{B}, \bar{C}]\}$

Let $A = \text{FALSE}$:

- Propagation: $\{[B, C], [\bar{B}, C], [\bar{B}, \bar{C}]\}$

Assume that the branching heuristic selects B :

- Let $B = \text{TRUE}$:

- Propagation: $\{[C], [\bar{C}]\}$

- By speed-up, the first clause consists of only one literal; we set $C = \text{TRUE}$

- Propagation: $\{[]\}$

- Conclusion: this branch is unsatisfiable

- Let $B = \text{FALSE}$:

- Propagation: $\{[C]\}$

- By speed-up, the first clause consists of only one literal; we set $C = \text{TRUE}$

KB: $\{[A, B, C], [\bar{A}, B], [\bar{B}, C], [\bar{B}, \bar{C}]\}$

Let $A = \text{FALSE}$:

- Propagation: $\{[B, C], [\bar{B}, C], [\bar{B}, \bar{C}]\}$

Assume that the branching heuristic selects B :

- Let $B = \text{TRUE}$:

- Propagation: $\{[C], [\bar{C}]\}$

- By speed-up, the first clause consists of only one literal; we set $C = \text{TRUE}$

- Propagation: $\{[]\}$

- Conclusion: this branch is unsatisfiable

- Let $B = \text{FALSE}$:

- Propagation: $\{[C]\}$

- By speed-up, the first clause consists of only one literal; we set $C = \text{TRUE}$

- Propagation: $\{\}$

KB: $\{[A, B, C], [\bar{A}, B], [\bar{B}, C], [\bar{B}, \bar{C}]\}$

Let $A = \text{FALSE}$:

- Propagation: $\{[B, C], [\bar{B}, C], [\bar{B}, \bar{C}]\}$

Assume that the branching heuristic selects B :

- Let $B = \text{TRUE}$:

- Propagation: $\{[C], [\bar{C}]\}$

- By speed-up, the first clause consists of only one literal; we set $C = \text{TRUE}$

- Propagation: $\{[]\}$

- Conclusion: this branch is unsatisfiable

- Let $B = \text{FALSE}$:

- Propagation: $\{[C]\}$

- By speed-up, the first clause consists of only one literal; we set $C = \text{TRUE}$

- Propagation: $\{\}$

- Conclusion: this branch is satisfiable; $A = \text{FALSE}$, $B = \text{FALSE}$, $C = \text{TRUE}$

Reasoning in CSP

The working of CSP solvers is similar to that of the DPLL algorithm

The power of DPLL comes from propagation

- Once the value of a literal is fixed, we can simplify/remove many clauses

In CSP, propagation is even more powerful:

- Constraints can be more complex and restrictive than SAT clauses
- Once some of the scope variables are assigned values, the solver can simplify the remaining problem

Example of constraint propagation

Consider the following CSP:

- Variables $x_1, x_2 \in \{1, 2, 3\}$ and $x_3 \in \{1, 2\}$
- Constraint Alldiff with scope $\{x_1, x_2, x_3\}$
- Some other variables and constraints. . .

At some point, the algorithm assigns $x_1 \leftarrow 2$

By propagation of Alldiff, we can immediately conclude that $x_3 = 1$ and $x_2 = 3$

Self-study exercise

Exercise

Convert the following formula into CNF

$$(A \rightarrow \neg B) \vee (\neg B \wedge C \wedge D)$$

Spoiler alert

Warning: answer in the following slides!

Solution: step 1

$$(A \rightarrow \neg B) \vee (\neg B \wedge C \wedge D)$$

Solution: step 1

$$\left(\underbrace{A}_{\alpha} \rightarrow \underbrace{\neg B}_{\beta} \right) \vee (\neg B \wedge C \wedge D)$$

Replace $(\alpha \rightarrow \beta)$ with $(\neg\alpha \vee \beta)$:

Solution: step 1

$$\underbrace{(A}_{\alpha} \rightarrow \underbrace{\neg B}_{\beta}) \vee (\neg B \wedge C \wedge D)$$

Replace $(\alpha \rightarrow \beta)$ with $(\neg\alpha \vee \beta)$:

$$\alpha = A \quad \beta = \neg B$$

$$(\neg A \vee \neg B) \vee (\neg B \wedge C \wedge D)$$

Solution: step 2

$$(\neg A \vee \neg B) \vee (\neg B \wedge C \wedge D)$$

Solution: step 2

$$\underbrace{(\neg A \vee \neg B)}_{\alpha} \vee (\neg B \wedge C \wedge D)$$

Replace $\alpha \vee (\beta \wedge \gamma)$ with $((\alpha \vee \beta) \wedge (\alpha \vee \gamma))$

Solution: step 2

$$\underbrace{(\neg A \vee \neg B)}_{\alpha} \vee (\neg B \wedge C \wedge D)$$

Replace $\alpha \vee (\beta \wedge \gamma)$ with $((\alpha \vee \beta) \wedge (\alpha \vee \gamma))$

$$((\neg A \vee \neg B) \vee \neg B) \wedge ((\neg A \vee \neg B) \vee (C \wedge D))$$

Solution: step 3

$$((\neg A \vee \neg B) \vee \neg B) \wedge ((\neg A \vee \neg B) \vee (C \wedge D))$$

Solution: step 3

$$((\neg A \vee \neg B) \vee \neg B) \wedge (\underbrace{(\neg A \vee \neg B)}_{\alpha} \vee (\underbrace{C}_{\beta} \wedge \underbrace{D}_{\gamma}))$$

Replace $\alpha \vee (\beta \wedge \gamma)$ with $(\alpha \vee \beta) \wedge (\alpha \vee \gamma)$

Solution: step 3

$$((\neg A \vee \neg B) \vee \neg B) \wedge (\underbrace{(\neg A \vee \neg B)}_{\alpha} \vee (\underbrace{C}_{\beta} \wedge \underbrace{D}_{\gamma}))$$

Replace $\alpha \vee (\beta \wedge \gamma)$ with $(\alpha \vee \beta) \wedge (\alpha \vee \gamma)$

$$((\neg A \vee \neg B) \vee \neg B) \wedge (((\neg A \vee \neg B) \vee C) \wedge ((\neg A \vee \neg B) \vee D))$$

Solution: step 4

$$((\neg A \vee \neg B) \vee \neg B) \wedge (((\neg A \vee \neg B) \vee C) \wedge ((\neg A \vee \neg B) \vee D))$$

Solution: step 4

$$((\neg A \vee \neg B) \vee \neg B) \wedge (((\neg A \vee \neg B) \vee C) \wedge ((\neg A \vee \neg B) \vee D))$$

Remove unnecessary brackets

Solution: step 4

$$((\neg A \vee \neg B) \vee \neg B) \wedge (((\neg A \vee \neg B) \vee C) \wedge ((\neg A \vee \neg B) \vee D))$$

Remove unnecessary brackets

$$(\neg A \vee \neg B \vee \neg B) \wedge (\neg A \vee \neg B \vee C) \wedge (\neg A \vee \neg B \vee D)$$

Solution: step 5

$$(\neg A \vee \neg B \vee \neg B) \wedge (\neg A \vee \neg B \vee C) \wedge (\neg A \vee \neg B \vee D)$$

Solution: step 5

$$(\neg A \vee \underbrace{\neg B}_{\alpha} \vee \underbrace{\neg B}_{\alpha}) \wedge (\neg A \vee \neg B \vee C) \wedge (\neg A \vee \neg B \vee D)$$

Replace $\alpha \vee \alpha$ with α

Solution: step 5

$$(\neg A \vee \underbrace{\neg B}_{\alpha} \vee \underbrace{\neg B}_{\alpha}) \wedge (\neg A \vee \neg B \vee C) \wedge (\neg A \vee \neg B \vee D)$$

Replace $\alpha \vee \alpha$ with α

$$(\neg A \vee \neg B) \wedge (\neg A \vee \neg B \vee C) \wedge (\neg A \vee \neg B \vee D)$$

Solution: step 5

$$(\neg A \vee \underbrace{\neg B}_{\alpha} \vee \underbrace{\neg B}_{\alpha}) \wedge (\neg A \vee \neg B \vee C) \wedge (\neg A \vee \neg B \vee D)$$

Replace $\alpha \vee \alpha$ with α

$$(\neg A \vee \neg B) \wedge (\neg A \vee \neg B \vee C) \wedge (\neg A \vee \neg B \vee D)$$

This formula is in CNF